\section*{PreCalculus}
\subsection*{Logarithm Properties}
\begin{eqlist}
	\item $\log_n(0) = \textit{Undefined}$
	\item $\log_n(1) = 0$
	\item $\log_n(n) = 1$
	\item $\log_n(n^x) = x$
	\item $n^{\log_n(x)} = x$
	\item $\log_n(x^r) = r\log_n(x) \neq \log_n^r(x) = (\log_n(x))^r$
	\item $\log_n(xy) = \log_n(x) + \log_n(y)$
	\item $\log_n\left(\frac{x}{y}\right) = \log_n(x) - \log_n(y)$
	\item $-\log_n(x) = \log_n\left(\frac{1}{x}\right)$
	\item $\frac{\log(x)}{\log(n)} = \log_n(x)$
\end{eqlist}


\subsection*{Absolute Value Properties} 
\begin{eqlist}
	\item $|ca| = c|a|, \quad \textit{if $c > 0$}$
	\item $|xy| = |x||y|$
	\item $|x^n| = |x|^n$
	\item $|a+b| \leq |a| + |b|$
	\item $|a|-|b| \leq |a-b|$ 
\end{eqlist}

\subsection*{Factorization}
\begin{eqlist}
	\item $x^3+3ax^2+3a^2x+a^3 = (x+a)^3$
	\item $x^3-3ax^2+3a^2x-a^3 = (x-a)^3$
	\item $x^3+a^3=(x+a)(x^2-ax+a^2)$
	\item $x^3-a^3=(x-a)(x^2+ax+a^2)$
	\item $x^{2n}-a^{2n}=(x^n-a^n)(x^n+a^n)$
\end{eqlist}
